## Entanglement Entropy

$$|\Psi_{e^+ + e^-} \rangle = \frac{1}{\sqrt {2}}\left(|\uparrow_{e^-}\downarrow_{e^{+}}\rangle + |\downarrow_{e^-}\uparrow_{e^{+}}\rangle\right)$$
$$\Psi = \sum_{nm}\Psi_{nm} \Psi_n \otimes\Phi+m$$

#### Density Matrix
$$\rho = \sum_n P_n |\Psi_n\rangle\langle\Psi_n|$$

#### Expectation Value
$$\langle\hat A\rangle = \sum_n\left(P_n\langle\Psi_n|\hat \Psi_n\rangle\right)=\mathsf{Tr}\{\hat A \rho\}$$

#### Von Neumann Entropy = Entanglement Entropy
$$S\equiv-k_B\sum_n P_n \ln P_n$$


## Bell's theorem

$$\symbf P \equiv \left(\frac{\hbar^2}{4}\right)^{-1}\langle\mathbf S_1 \cdot \mathbf a \mathbf S_2 \cdot \mathbf b \rangle$$
$$\symbf P =- \left(\frac{\hbar^2}{4}\right)^{-1}\langle\mathbf S_1 \cdot \mathbf a \mathbf S_1 \cdot \mathbf b \rangle$$

$$\mathbf S \cdot \mathbf a \mathbf S \cdot \mathbf b=\sum_{i,j}S_i S_j a_i b_j$$
$$S_i S_j = \frac{\hbar^2}{4}\delta_{ij}+i\frac{\hbar}{2}\epsilon{ijk}S_k$$
$$=\frac{\hbar^2}{4}\mathbf a \cdot \mathbf b + i\frac{\hbar}{2}\mathbf a \mathbf b$$

#### Pauli matrix
$$\delta = \dots$$

Therefore
$$\symbf P = -\mathbf a \cdot \mathbf b$$

#### In the Hidden Variable Theory
$$\symbf P (\mathbf a, \mathbf b) = -\int \rho (\lambda) A(\mathbf a, \lambda), A(\mathbf b, \lambda)d\lambda$$

#### Bell's Inequality
$$\mathbf P(\mathbf a, \mathbf b)-\mathbf P(\mathbf a, \mathbf c)=-\int\rho(\lambda)\left[A(\mathbf a, \lambda)+A(\mathbf b, \lambda)-A(\mathbf a, \lambda)A(\mathbf c, \lambda)\right]$$
$$=-\int \rho(\lambda) \left[1-A(\mathbf b,lambda)A(\mathbf c, \lambda)\right]A(\mathbf a, \lambda)A(\mathbf b, \lambda)$$

cf: $$1 = (A(\mathbf b,\lambda))^2$$

By Schwarz Inequality:

$$\left|P(\mathbf a, \mathbf b) - P(\mathbf a, \mathbf c)\right| = \int \rho(\lambda)\left[1-A(\mathbf b, \lambda)A(\mathbf a, c)\right]d\lambda$$
$$=1-\int\rho(\lambda)A(\mathbf b, \lambda)A(\mathbf a, \lambda)d\lambda$$
$$=1+P(\mathbf b, \mathbf c)$$
## Violation of Bell's Inequality

$$P(\mathbf a, \mathbf b) = - \mathbf a\cdot\mathbf b = 0$$
$$P(\mathbf a, \mathbf c) = \frac{1}{\sqrt 2}$$
$$\left|P(\mathbf a, \mathbf b) - P(\mathbf a, \mathbf c)\right| = \frac{1}{\sqrt}>1+P(\mathbf b, \mathbf c) =\frac{\sqrt 2 - 1}{\sqrt 2}$$

## No clone theory
